Superposition_Calculus/Term_Rewrite_System.thy
@@ -1,0 +1,68 @@
+theory Term_Rewrite_System
+  imports
+    (* Theories from the AFP *)
+    "Knuth_Bendix_Order.Subterm_and_Context"
+begin
+
+text \<open>This is for ground terms only!\<close>
+
+definition compatible_with_ctxt :: "(('f, 'v) term \<times> ('f, 'v) term) set \<Rightarrow> bool" where
+  "compatible_with_ctxt I \<longleftrightarrow> (\<forall>ctxt t t'. (t, t') \<in> I \<longrightarrow> (ctxt\<langle>t\<rangle>, ctxt\<langle>t'\<rangle>) \<in> I)"
+
+lemma compatible_with_ctxtD:
+  "compatible_with_ctxt I \<Longrightarrow> (t, t') \<in> I \<Longrightarrow> (ctxt\<langle>t\<rangle>, ctxt\<langle>t'\<rangle>) \<in> I"
+  by (simp add: compatible_with_ctxt_def)
+
+lemma compatible_with_ctxt_symcl:
+  assumes "compatible_with_ctxt I"
+  shows "compatible_with_ctxt (I\<^sup>\<leftrightarrow>)"
+  unfolding compatible_with_ctxt_def
+proof (intro allI impI)
+  fix ctxt t t'
+  assume "(t, t') \<in> I\<^sup>\<leftrightarrow>"
+  then show "(ctxt\<langle>t\<rangle>, ctxt\<langle>t'\<rangle>) \<in> I\<^sup>\<leftrightarrow>"
+  proof (induction ctxt arbitrary: t t')
+    case Hole
+    then show ?case by simp
+  next
+    case (More f ts1 ctxt ts2)
+    then show ?case
+      using assms[unfolded compatible_with_ctxt_def, rule_format]
+      by blast
+  qed
+qed
+
+lemma compatible_with_ctxt_rtrancl:
+  assumes "compatible_with_ctxt I"
+  shows "compatible_with_ctxt (I\<^sup>*)"
+  unfolding compatible_with_ctxt_def
+proof (intro allI impI)
+  fix ctxt t t'
+  assume "(t, t') \<in> I\<^sup>*"
+  then show "(ctxt\<langle>t\<rangle>, ctxt\<langle>t'\<rangle>) \<in> I\<^sup>*"
+  proof (induction t' rule: rtrancl_induct)
+    case base
+    then show ?case
+      by simp
+  next
+    case (step y z)
+    then show ?case
+      using assms[unfolded compatible_with_ctxt_def, rule_format]
+      by (meson rtrancl.rtrancl_into_rtrancl)
+  qed
+qed
+lemma compatible_with_ctxt_conversion:
+  assumes "compatible_with_ctxt I"
+  shows "compatible_with_ctxt (I\<^sup>\<leftrightarrow>\<^sup>*)"
+  by (simp add: assms compatible_with_ctxt_rtrancl compatible_with_ctxt_symcl conversion_def)
+
+definition rewrite_inside_ctxt where
+  "rewrite_inside_ctxt E = {(ctxt\<langle>s\<rangle>, ctxt\<langle>t\<rangle>) | ctxt s t. (s, t) \<in> E}"
+
+lemma compatible_with_ctxt_rewrite_inside_ctxt: "compatible_with_ctxt (rewrite_inside_ctxt E)"
+  unfolding compatible_with_ctxt_def rewrite_inside_ctxt_def
+  unfolding mem_Collect_eq
+  by (metis Pair_inject ctxt_ctxt)
+    
+
+end
